draft

theories/simulang/simple_inv/examples/paper.v
@@ -50,31 +50,6 @@ Section pre_allocated.
 End pre_allocated.
 
 
-Section spec_preservation.
-  Variable source_allocated: list loc.
-
-  Variable mapping: gmap loc loc.
-  Variable heap_s: gset loc.
-  Variable heap_t: gset loc.
-
-  Definition state := loc -> val.
-  Variable mem_s: state.
-  Variable mem_t: state.
-
-  Definition wf_mapping : Prop :=
-    heap_s ⊆ dom mapping.
-
-  Definition equivalence: Prop :=
-    wf_mapping ->
-    (forall add_s, add_s ∈ heap_s ->
-      match mapping !! add_s with
-      | Some add_t => mem_s add_s = mem_t add_t
-      | None => False
-      end).
-
-End spec_preservation.
-
-
 (* define the equivalence relationship *)
 Section pre_allocated.
 
@@ -82,20 +57,20 @@ Section pre_allocated.
 
   Variable l_s l_t : loc.
 
-  Definition target : expr :=
+  Definition c_target : expr :=
     Call f#"f" #24;;
     #42.
 
-  Definition source : expr :=
+  Definition c_source : expr :=
     Call f#"f" #24;;
     !#l_s.
 
-  Lemma relate_s_t π:
+  Lemma relate_s_t_c π:
     ⊢ {{{ l_t ↦t #42 ∗ l_s ↦s #42 }}} 
-        target ⪯[π] source
+        c_target ⪯[π] c_source
       {{{ lift_post (λ v_t v_s, ⌜v_t = v_s⌝ ∗ l_t ↦t #42 ∗ l_s ↦s #42) }}}.
   Proof.
-    unfold source. unfold target.
+    unfold c_source. unfold c_target.
     (* introduce the pre-condition *)
     iIntros "!> [Hlt Hls]". 
     (* continue with a pair of sub-expr, here is the call *)
