theories/simulang/simple_inv/examples/uberobj/lang_core.v
@@ -1,0 +1,124 @@
+From stdpp Require Import gmap.
+From simuliris.simulation Require Import language .
+From simuliris.simulang Require Import lang notation tactics class_instances.
+From simuliris.simulation Require Import slsls lifting .
+From iris.proofmode Require Import proofmode.
+From iris.prelude Require Import options.
+
+From simuliris.simulang Require Import hoare behavior.
+From simuliris.simulang.simple_inv Require Import inv adequacy.
+
+Definition hl_halted (e: expr) : option val := to_val e.
+
+Definition hl_at_external (e: expr) : option (string * val) :=
+  match (decompose_expr [] e) with
+  | Some (K, Call e1 e2) => 
+      match ((to_val e1), (to_val e2)) with
+      (* and the parameter has been a value *)
+      | (Some (LitV (LitFn f)), Some argv) => Some (f, argv)
+      | _ => None
+      end
+  | _ => None
+  end.
+
+Definition hl_after_external (vret: option val) (e: expr) : option expr :=
+  match vret with
+  | Some v => 
+      match (decompose_expr [] e) with
+      | Some (K, Call e1 e2) => 
+          match ((to_val e1), (to_val e2)) with
+          | (Some (LitV (LitFn f)), Some argv) => Some (fill K (of_val v))
+          | _ => None
+          end
+      | _ => None
+      end
+  | None => None
+  end.
+
+Notation uobj_id := nat.
+(* how to support pointer to pointer *)
+Definition closed (locs : list loc) (m : state) : Prop :=
+  forall (l: loc) (l': loc) (ls: lock_state),
+    In l locs ->
+    m.(heap) !! l = Some (ls, LitV (LitLoc l')) ->
+    In l' locs.
+
+Definition sublist (l1 l2 : list loc) : Prop :=
+  forall x, In x l1 -> In x l2.
+
+Section specs.
+
+  (* =====================================================================================
+                                    source level definition 
+     ===================================================================================== *)
+  Variable functions : prog.
+  Inductive hl_prim_step : expr -> state -> expr -> state -> Prop :=
+    | hl_prim_step_base : 
+        forall e σ σ' e' efs,
+          prim_step functions e σ e' σ' efs ->
+          hl_prim_step e σ e' σ'.
+
+  (* compartmentally pre-allocated heap space for uids *)
+  Variable heap_by_uid : uobj_id -> list loc.  
+  Variable uid : uobj_id.
+  (* fname -> (isCasm func * (pre-cond, post-cond)) *)
+  Variable ext_funcs : string -> option (bool * ((state -> Prop) * (state -> Prop))). 
+
+  Definition R_relation (m: state) (m': state) (modified: bool) : Prop :=
+    closed (heap_by_uid uid) m' 
+    /\ subseteq (dom m.(heap)) (dom m'.(heap))
+    /\ (not modified -> forall l, In l (heap_by_uid uid) -> m.(heap) !! l = m'.(heap) !! l).
+
+  Inductive respecting_the_specs (e : expr) (m : state) (Q : state -> Prop) : Prop :=
+    | rts_base : 
+      forall m', R_relation m m' false ->
+      (* internal steps *)
+      ((forall (e' : expr) (m'' : state), hl_prim_step e m' e' m'' -> respecting_the_specs e' m'' Q )
+        (* halted case *)
+        /\ (not (eq (hl_halted e) None) -> Q m')
+        (* external call case *)
+        /\ (forall fname argv is_casm (pre_spec : state -> Prop) m'' (post_spec : state -> Prop) vret e',
+          (* m_extra satisfied the pre_sped of the external call *)
+          hl_at_external e = Some (fname, argv)
+          -> Some (is_casm, (pre_spec, post_spec) ) = ext_funcs fname
+          -> pre_spec m'
+          -> R_relation m' m'' is_casm
+          -> post_spec m''
+          -> hl_after_external (Some vret) e = Some e'
+          -> respecting_the_specs e' m Q) 
+      ) -> respecting_the_specs e m Q.
+
+  (* =====================================================================================
+                                    memory mapping 
+     ===================================================================================== *)
+  Variable mapping: gmap loc loc.
+  Variable heap_s: gset loc.
+  Variable heap_t: gset loc.
+
+
+  Definition wf_mapping : Prop :=
+    heap_s ⊆ dom mapping.
+
+  Definition equivalence s_mem t_mem: Prop :=
+    wf_mapping ->
+    (forall add_s, add_s ∈ heap_s ->
+      match mapping !! add_s with
+      | Some add_t => s_mem.(heap) !! add_s = t_mem.(heap) !! add_t
+      | None => False
+      end).
+
+  (* =====================================================================================
+                                   spec preservation 
+     ===================================================================================== *)
+  Context `{!simpleGS Σ}.
+  Lemma preservation_of_respecting_the_specs s_exp t_exp s_mem t_mem Q :
+      (⊢ {{{ ⌜equivalence s_mem t_mem⌝  }}} 
+          t_exp ⪯[uid] s_exp
+        {{{ lift_post (λ v_t v_s, ⌜equivalence s_mem t_mem⌝) }}})
+      -> respecting_the_specs s_exp s_mem Q
+      -> respecting_the_specs t_exp t_mem Q.
+  Proof.
+  Admitted.
+
+
+End specs.
